VeriTile/Triton/Memory/Typing/Contracts.lean
@@ -165,6 +165,13 @@ def Stmt.RespectsRegionTyping (Γ : RegionTyping) : Stmt → Prop
   | @Stmt.atomicAdd dtype _ _ mem val mask =>
       mem.RespectsRegionTyping Γ dtype ∧
       val.RespectsRegionTyping Γ ∧ mask.RespectsRegionTyping Γ
+  | .atomicRMW _ dtype _ mem input extraInput mask _ =>
+      mem.RespectsRegionTyping Γ dtype ∧
+      input.RespectsRegionTyping Γ ∧
+      (match extraInput with
+        | none => True
+        | some extra => extra.RespectsRegionTyping Γ) ∧
+      mask.RespectsRegionTyping Γ
   | .forLoop _ _ body => StmtList.RespectsRegionTyping Γ body
   | .ifThen cond body =>
       cond.RespectsRegionTyping Γ ∧ StmtList.RespectsRegionTyping Γ body
